src/SDK/Serialize.dfy
@@ -104,11 +104,9 @@ module Serialize {
     var len := wr.WriteUInt16(kvPairsLength as uint16);
 
     totalWritten := totalWritten + len;
-    if kvPairsLength == 0 {
-      return Success(totalWritten);
-    }
 
-    len := wr.WriteUInt16(|kvPairs| as uint16);
+
+    len :- SerializeKVPairs(wr, kvPairs);
     totalWritten := totalWritten + len;
 
     var j := 0;
@@ -137,6 +135,58 @@ module Serialize {
       j := j + 1;
     }
     
+    return Success(totalWritten);
+  }
+
+  // ----- SerializeKVPairs -----
+
+  method SerializeKVPairs(wr: Streams.StringWriter, kvPairs: Materials.EncryptionContext) returns (ret: Result<nat>)
+    requires wr.Valid() && Msg.ValidKVPairs(kvPairs)
+    modifies wr`data
+    ensures wr.Valid() && Msg.ValidKVPairs(kvPairs)
+    ensures match ret
+      case Success(totalWritten) =>
+        var serAAD := Msg.KVPairsToSeq(kvPairs);
+        var initLen := old(|wr.data|);
+        && totalWritten == |serAAD|
+        && initLen + totalWritten == |wr.data|
+        && wr.data == old(wr.data) + serAAD
+      case Failure(e) => true
+  {
+    var totalWritten := 0;
+
+    if |kvPairs| == 0 {
+      return Success(totalWritten);
+    }
+
+    var len :- wr.WriteUInt16(|kvPairs| as uint16);
+    totalWritten := totalWritten + len;
+
+    var j := 0;
+    ghost var n := |kvPairs|;
+    while j < |kvPairs|
+      invariant j <= n == |kvPairs|
+      invariant wr.data ==
+        old(wr.data) +
+        UInt16ToSeq(n as uint16) +
+        Msg.KVPairEntriesToSeq(kvPairs, 0, j)
+      invariant totalWritten == 2 + |Msg.KVPairEntriesToSeq(kvPairs, 0, j)|
+    {
+      len :- wr.WriteUInt16(|kvPairs[j].0| as uint16);
+      totalWritten := totalWritten + len;
+
+      len :- wr.WriteSeq(kvPairs[j].0);
+      totalWritten := totalWritten + len;
+
+      len :- wr.WriteUInt16(|kvPairs[j].1| as uint16);
+      totalWritten := totalWritten + len;
+
+      len :- wr.WriteSeq(kvPairs[j].1);
+      totalWritten := totalWritten + len;
+
+      j := j + 1;
+    }
+
     return Success(totalWritten);
   }
 
